ocaml/fstar-lib/generated/FStar_Syntax_Util.ml
@@ -4855,18 +4855,35 @@ let (contains_strictly_positive_attribute :
                FStar_Parser_Const.binder_strictly_positive_attr
              -> true
          | uu___ -> false) attrs
+let (contains_unused_attribute :
+  FStar_Syntax_Syntax.attribute Prims.list -> Prims.bool) =
+  fun attrs ->
+    FStar_Compiler_Util.for_some
+      (fun a ->
+         match a.FStar_Syntax_Syntax.n with
+         | FStar_Syntax_Syntax.Tm_fvar fv when
+             FStar_Syntax_Syntax.fv_eq_lid fv
+               FStar_Parser_Const.binder_unused_attr
+             -> true
+         | uu___ -> false) attrs
 let (parse_positivity_attributes :
   FStar_Syntax_Syntax.attribute Prims.list ->
     (FStar_Syntax_Syntax.positivity_qualifier FStar_Pervasives_Native.option
       * FStar_Syntax_Syntax.attribute Prims.list))
   =
   fun attrs ->
-    let uu___ = contains_strictly_positive_attribute attrs in
+    let uu___ = contains_unused_attribute attrs in
     if uu___
     then
-      ((FStar_Pervasives_Native.Some
-          FStar_Syntax_Syntax.BinderStrictlyPositive), attrs)
-    else (FStar_Pervasives_Native.None, attrs)
+      ((FStar_Pervasives_Native.Some FStar_Syntax_Syntax.BinderUnused),
+        attrs)
+    else
+      (let uu___2 = contains_strictly_positive_attribute attrs in
+       if uu___2
+       then
+         ((FStar_Pervasives_Native.Some
+             FStar_Syntax_Syntax.BinderStrictlyPositive), attrs)
+       else (FStar_Pervasives_Native.None, attrs))
 let (encode_positivity_attributes :
   FStar_Syntax_Syntax.positivity_qualifier FStar_Pervasives_Native.option ->
     FStar_Syntax_Syntax.attribute Prims.list ->
@@ -4874,30 +4891,42 @@ let (encode_positivity_attributes :
   =
   fun pqual ->
     fun attrs ->
-      let uu___ =
-        (pqual = FStar_Pervasives_Native.None) ||
-          (contains_strictly_positive_attribute attrs) in
-      if uu___
-      then attrs
-      else
-        (let qual =
-           match pqual with
-           | FStar_Pervasives_Native.Some
-               (FStar_Syntax_Syntax.BinderStrictlyPositive) ->
-               let uu___2 =
-                 let uu___3 =
-                   FStar_Syntax_Syntax.lid_as_fv
-                     FStar_Parser_Const.binder_strictly_positive_attr
-                     (FStar_Syntax_Syntax.Delta_constant_at_level
-                        Prims.int_zero) FStar_Pervasives_Native.None in
-                 FStar_Syntax_Syntax.fv_to_tm uu___3 in
-               [uu___2]
-           | FStar_Pervasives_Native.Some (FStar_Syntax_Syntax.BinderUnused)
-               -> [] in
-         FStar_Compiler_List.op_At qual attrs)
+      match pqual with
+      | FStar_Pervasives_Native.None -> attrs
+      | FStar_Pervasives_Native.Some
+          (FStar_Syntax_Syntax.BinderStrictlyPositive) ->
+          let uu___ = contains_strictly_positive_attribute attrs in
+          if uu___
+          then attrs
+          else
+            (let uu___2 =
+               let uu___3 =
+                 FStar_Syntax_Syntax.lid_as_fv
+                   FStar_Parser_Const.binder_strictly_positive_attr
+                   (FStar_Syntax_Syntax.Delta_constant_at_level
+                      Prims.int_zero) FStar_Pervasives_Native.None in
+               FStar_Syntax_Syntax.fv_to_tm uu___3 in
+             uu___2 :: attrs)
+      | FStar_Pervasives_Native.Some (FStar_Syntax_Syntax.BinderUnused) ->
+          let uu___ = contains_unused_attribute attrs in
+          if uu___
+          then attrs
+          else
+            (let uu___2 =
+               let uu___3 =
+                 FStar_Syntax_Syntax.lid_as_fv
+                   FStar_Parser_Const.binder_unused_attr
+                   (FStar_Syntax_Syntax.Delta_constant_at_level
+                      Prims.int_zero) FStar_Pervasives_Native.None in
+               FStar_Syntax_Syntax.fv_to_tm uu___3 in
+             uu___2 :: attrs)
 let (is_binder_strictly_positive : FStar_Syntax_Syntax.binder -> Prims.bool)
   =
   fun b ->
     b.FStar_Syntax_Syntax.binder_positivity =
       (FStar_Pervasives_Native.Some
          FStar_Syntax_Syntax.BinderStrictlyPositive)
+let (is_binder_unused : FStar_Syntax_Syntax.binder -> Prims.bool) =
+  fun b ->
+    b.FStar_Syntax_Syntax.binder_positivity =
+      (FStar_Pervasives_Native.Some FStar_Syntax_Syntax.BinderUnused)
