ocaml/fstar-lib/generated/FStar_TypeChecker_TcTerm.ml
@@ -6244,37 +6244,65 @@ and (tc_abs :
                               FStar_Syntax_Util.abs bs1 body2 uu___7 in
                             FStar_Compiler_List.iter
                               (fun b ->
-                                 let uu___8 =
-                                   (FStar_Syntax_Util.is_binder_strictly_positive
-                                      b)
-                                     &&
-                                     (let uu___9 =
-                                        FStar_Options.no_positivity () in
-                                      Prims.op_Negation uu___9) in
+                                 let uu___8 = FStar_Options.no_positivity () in
                                  if uu___8
-                                 then
-                                   let r =
-                                     FStar_TypeChecker_Positivity.name_strictly_positive_in_type
-                                       envbody1
-                                       b.FStar_Syntax_Syntax.binder_bv body2 in
-                                   (if Prims.op_Negation r
-                                    then
-                                      let uu___9 =
-                                        let uu___10 =
-                                          let uu___11 =
-                                            FStar_Syntax_Print.binder_to_string
-                                              b in
-                                          FStar_Compiler_Util.format1
-                                            "Binder %s is marked strictly positive, but its use in the definition is not"
-                                            uu___11 in
-                                        (FStar_Errors_Codes.Error_InductiveTypeNotSatisfyPositivityCondition,
-                                          uu___10) in
-                                      let uu___10 =
-                                        FStar_Syntax_Syntax.range_of_bv
-                                          b.FStar_Syntax_Syntax.binder_bv in
-                                      FStar_Errors.raise_error uu___9 uu___10
-                                    else ())
-                                 else ()) bs1;
+                                 then ()
+                                 else
+                                   ((let uu___11 =
+                                       (FStar_Syntax_Util.is_binder_unused b)
+                                         &&
+                                         (let uu___12 =
+                                            FStar_TypeChecker_Positivity.name_unused_in_type
+                                              envbody1
+                                              b.FStar_Syntax_Syntax.binder_bv
+                                              body2 in
+                                          Prims.op_Negation uu___12) in
+                                     if uu___11
+                                     then
+                                       let uu___12 =
+                                         let uu___13 =
+                                           let uu___14 =
+                                             FStar_Syntax_Print.binder_to_string
+                                               b in
+                                           FStar_Compiler_Util.format1
+                                             "Binder %s is marked unused, but its use in the definition is not"
+                                             uu___14 in
+                                         (FStar_Errors_Codes.Error_InductiveTypeNotSatisfyPositivityCondition,
+                                           uu___13) in
+                                       let uu___13 =
+                                         FStar_Syntax_Syntax.range_of_bv
+                                           b.FStar_Syntax_Syntax.binder_bv in
+                                       FStar_Errors.raise_error uu___12
+                                         uu___13
+                                     else ());
+                                    (let uu___11 =
+                                       (FStar_Syntax_Util.is_binder_strictly_positive
+                                          b)
+                                         &&
+                                         (let uu___12 =
+                                            FStar_TypeChecker_Positivity.name_strictly_positive_in_type
+                                              envbody1
+                                              b.FStar_Syntax_Syntax.binder_bv
+                                              body2 in
+                                          Prims.op_Negation uu___12) in
+                                     if uu___11
+                                     then
+                                       let uu___12 =
+                                         let uu___13 =
+                                           let uu___14 =
+                                             FStar_Syntax_Print.binder_to_string
+                                               b in
+                                           FStar_Compiler_Util.format1
+                                             "Binder %s is marked strictly positive, but its use in the definition is not"
+                                             uu___14 in
+                                         (FStar_Errors_Codes.Error_InductiveTypeNotSatisfyPositivityCondition,
+                                           uu___13) in
+                                       let uu___13 =
+                                         FStar_Syntax_Syntax.range_of_bv
+                                           b.FStar_Syntax_Syntax.binder_bv in
+                                       FStar_Errors.raise_error uu___12
+                                         uu___13
+                                     else ()))) bs1;
                             (let uu___8 =
                                match tfun_opt with
                                | FStar_Pervasives_Native.Some t ->
