ulib/FStar.Pervasives.fst
@@ -176,6 +176,8 @@ let primitive_extraction = ()
 
 let strictly_positive = ()
 
+let unused = ()
+
 let no_auto_projectors = ()
 
 let no_subtyping = ()
